src/lowparse/steel_st_array/LowParse.Steel.StdInt.fsti
@@ -59,6 +59,11 @@ val size_div (x y: size_t) : Pure size_t
   (ensures (fun z -> size_v z == size_v x / size_v y))
 
 inline_for_extraction
+val size_mod (x y: size_t) : Pure size_t
+  (requires (size_v y > 0))
+  (ensures (fun z -> size_v z == size_v x % size_v y))
+
+inline_for_extraction
 val size_le (x y: size_t) : Pure bool
   (requires True)
   (ensures (fun z -> z == (size_v x <= size_v y)))
